src/Cipher.dfy
@@ -60,8 +60,10 @@ module Cipher {
 
     method EncryptBody(outp: ByteBuf, inp: ByteCursor, seqno: nat, iv: array<byte>, key: content_key, tag: array<byte>, body_frame_type: FrameType)
       returns (result: Outcome, message_id: array<byte>)
+      ensures fresh(message_id)
     {
       // TODO
+      message_id := new [][];  // TODO
     }
 
   }
