src/Session.dfy
@@ -86,16 +86,29 @@ module Session {
       match state
       case Config =>
         data_so_far == 0
-      case Error(r) => r != AWS_OP_SUCCESS
+      case Error(r) =>
+        r != AWS_OP_SUCCESS
       case Done => true
+      // decryption
       case ReadHeader => true
       case UnwrapKey => true
       case DecryptBody => true
       case CheckTrailer => true
-      case GenKey => true
-      case WriteHeader => true
-      case EncryptBody => true
-      case WriteTrailer => true
+      // encryption
+      case GenKey =>
+        data_so_far == 0
+      case WriteHeader =>
+        alg_props != null && content_key != null &&
+        data_so_far == 0 &&
+        header_copy != null && header_size <= header_copy.Length &&
+        (alg_props.signature_len != 0 ==> signctx != null)
+      case EncryptBody =>
+        alg_props != null && content_key != null &&
+        (precise_size.Some? ==> data_so_far <= precise_size.get) &&
+        (alg_props.signature_len != 0 ==> signctx != null)
+      case WriteTrailer =>
+        alg_props != null &&
+        (alg_props.signature_len != 0 ==> signctx != null)
     }
 
     constructor FromCMM(mode: ProcessingMode, cmm: CMM)
@@ -160,57 +173,38 @@ module Session {
       requires outp != inp && inlen <= inp.Length && outlen <= outp.Length
       modifies this, header, outp
       modifies header, header.iv.a, header.auth_tag.a, header.message_id
-      /**
-      ensures Valid() && message_size == old(message_size)
-      ensures in_bytes_read <= inlen && out_bytes_written <= outlen
-      ensures result != AWS_OP_SUCCESS ==>
-                input_consumed == old(input_consumed) &&
-                forall i :: 0 <= i < outlen ==> outp[i] == 0
+      ensures Valid()
+      ensures state.Error? || state == Done
       ensures result == AWS_OP_SUCCESS ==> state == Done
-      ensures result == AWS_OP_SUCCESS ==>
-                input_consumed == old(input_consumed) + in_bytes_read &&
-                in_bytes_read == inlen
-      ensures result == AWS_OP_SUCCESS && mode == EncryptMode ==>
-                outp[..out_bytes_written] == Math.Encrypt(inp[..in_bytes_read])
-      ensures result == AWS_OP_SUCCESS && mode == DecryptMode ==>
-                outp[..out_bytes_written] == Math.Decrypt(inp[..in_bytes_read])
-      **/
+      ensures in_bytes_read <= inlen && out_bytes_written <= outlen
+      ensures result != AWS_OP_SUCCESS ==> forall i :: 0 <= i < outlen ==> outp[i] == 0
     {
       var output := ByteBufFromArray(outp, outlen);
       var input := ByteCursorFromArray(inp, inlen);
 
       label tryit: {
         // ----- Config
-        assert state == Config;
-        var remaining_space := ByteBufFromRemaining(output);
         state := GenKey;
 
         // ----- GenKey
-        assert state == GenKey;
         result := priv_try_gen_key();
         if result != AWS_OP_SUCCESS { break tryit; }
 
         // ----- WriteHeader
-        assert state == WriteHeader;
         output := priv_try_write_header(output);
-        if state != EncryptBody { result := AWS_OP_ERR; break tryit; }
+        if state != EncryptBody { result := AWS_OP_ERR; break tryit; }  // output buffer is not large enough to hold header
 
         // ----- EncryptBody
-        assert state == EncryptBody;
-        assert header == old(header);
         result, output, input := priv_try_encrypt_body(output, input);
         if result != AWS_OP_SUCCESS { break tryit; }
         if state != WriteTrailer { result := AWS_OP_ERR; break tryit; }
 
         // ----- WriteTrailer
-        assert state == WriteTrailer;
-        assert output.a == outp;  // DEBUG
         result, output := priv_write_trailer(output);
         if result != AWS_OP_SUCCESS { break tryit; }
         if state != Done { result := AWS_OP_ERR; break tryit; }
 
         // ----- Done
-        assert state == Done;
       }
       assert result == AWS_OP_SUCCESS ==> state == Done;
 
@@ -225,12 +219,14 @@ module Session {
       }
     }
 
-    /*****
     method Process(outp: array<byte>, outlen: nat, inp: array<byte>, inlen: nat) returns (result: Outcome, out_bytes_written: nat, in_bytes_read: nat)
       requires Valid()
       requires outp != inp && inlen <= inp.Length && outlen <= outp.Length
-      modifies this, outp
-      ensures Valid() && message_size == old(message_size)
+      requires mode == EncryptMode && state !in { ReadHeader, UnwrapKey, DecryptBody, CheckTrailer }  // TODO: should also support DecryptMode
+      modifies this, header, header.message_id, header.iv.a, header.auth_tag.a, outp
+      ensures Valid()
+      /**
+      ensures message_size == old(message_size)
       ensures in_bytes_read <= inlen && out_bytes_written <= outlen
       ensures result != AWS_OP_SUCCESS ==>
                 input_consumed == old(input_consumed) &&
@@ -242,19 +238,30 @@ module Session {
                 outp[..out_bytes_written] == Math.Encrypt(inp[..in_bytes_read])
       ensures result == AWS_OP_SUCCESS && mode == DecryptMode ==>
                 outp[..out_bytes_written] == Math.Decrypt(inp[..in_bytes_read])
+      **/
     {
-      var output := ByteBuf(0, outp, 0, outlen);
-      var input := ByteCursor(inlen, inp, 0);
+      var output := ByteBufFromArray(outp, outlen);
+      var input := ByteCursorFromArray(inp, inlen);
 
       while true
         invariant Valid()
-        invariant output.len <= outlen && input.ptr <= inlen
-        invariant output.len <= output.capacity
-        decreases outlen - output.len, inlen - input.ptr, if state == Config then 1 else 0
+        invariant state !in { ReadHeader, UnwrapKey, DecryptBody, CheckTrailer }  // TODO: should also support DecryptMode
+        invariant GoodByteBuf(output) && GoodByteCursor(input)
+        invariant output.a == outp && input.a == inp
+        invariant header == old(header) || fresh(header)
+        invariant header.message_id == old(header.message_id) || fresh(header.message_id)
+        invariant header.iv.a == old(header.iv.a) || fresh(header.iv.a)
+        invariant header.auth_tag.a == old(header.auth_tag.a) || fresh(header.auth_tag.a)
+        decreases
+          if state == Config then 20
+          else if state == GenKey then 18
+          else if state == WriteHeader then 16
+          else if state == EncryptBody then 14
+          else if state == WriteTrailer then 12
+          else 0,
+          output.end - output.start - output.len
       {
-        var prior_state, old_inp := state, input.ptr;
-
-        var remaining_space := byte_buf_from_empty_array(output.enclosing_buffer, output.buffer_start_offset + output.len, output.capacity - output.len);
+        var prevState, prevOutput, prevInput := state, output, input;
 
         match state {
           case Config =>
@@ -273,32 +280,35 @@ module Session {
           case GenKey =>
             result := priv_try_gen_key();
           case WriteHeader =>
-            remaining_space := priv_try_write_header(remaining_space);
-            result := AWS_OP_SUCCESS;
+            output := priv_try_write_header(output);
           case EncryptBody =>
-            result := priv_try_encrypt_body(remaining_space, input);
-          case WriterTrailer =>
-            result := priv_write_trailer(remaining_space);
+            result, output, input := priv_try_encrypt_body(output, input);
+          case WriteTrailer =>
+            result, output := priv_write_trailer(output);
         }
-        var made_progress := remaining_space.len != 0 || input.ptr != old_inp || prior_state != state;
-
-        output := output.(len := output.len + remaining_space.len);
-        if result != AWS_OP_SUCCESS || !made_progress {
+        if result != AWS_OP_SUCCESS {
+          break;
+        }
+        if state == prevState &&
+          output.start + output.len == prevOutput.start + prevOutput.len &&
+          input.start + input.len == prevInput.start + prevInput.len {
+          // the iteration made no progress
           break;
         }
       }
 
-      out_bytes_written, in_bytes_read := output.len, input.ptr;
+      out_bytes_written, in_bytes_read := output.len, input.len;
 
       if result != AWS_OP_SUCCESS {
-        state := Error(result);
         forall i | 0 <= i < outlen {
           outp[i] := 0;
         }
         out_bytes_written := 0;
+        if !state.Error? {
+          state := Error(result);
+        }
       }
     }
-    *****/
 
     predicate method IsDone()
       requires Valid()
@@ -318,16 +328,11 @@ module Session {
 
     method priv_try_gen_key() returns (result: Outcome)
       requires Valid() && state == GenKey
-      modifies this
-      modifies header.iv.a, header.auth_tag.a
-      modifies header, header.message_id
+      modifies this, header, header.message_id
       ensures Valid()
-      ensures unchanged(`data_so_far, `header)
+      ensures unchanged(`header, header`message_id)
       ensures result == AWS_OP_SUCCESS ==> state == WriteHeader
-      ensures result == AWS_OP_SUCCESS ==>
-        alg_props != null && content_key != null &&
-        (alg_props.signature_len != 0 ==> signctx != null) &&
-        header_copy != null && header_size <= header_copy.Length
+      ensures result == AWS_OP_SUCCESS ==> fresh(header.iv.a) && fresh(header.auth_tag.a)
     {
       var materials, data_key := null, null;
       label tryit: {
@@ -421,6 +426,7 @@ module Session {
       ensures materials.unencrypted_data_key == old(materials.unencrypted_data_key)
       ensures GoodByteBuf(header.iv) && GoodByteBuf(header.auth_tag)
       ensures fresh(header.iv.a) && fresh(header.auth_tag.a)
+      ensures unchanged(header`message_id)
       ensures header.iv.len == alg_props.iv_len && header.auth_tag.len == alg_props.tag_len
     {
       header.alg_id := alg_props.alg_id;
@@ -508,11 +514,12 @@ module Session {
     }
 
     method priv_try_write_header(output: ByteBuf) returns (output': ByteBuf)
+      requires Valid() && state == WriteHeader
       requires GoodByteBuf(output)
-      requires header_copy != null && header_size <= header_copy.Length
       modifies `output_size_estimate, `state, output.a
-      ensures GoodByteBuf(output') && output'.a == output.a
+      ensures Valid()
       ensures state == old(state) || state == EncryptBody
+      ensures ByteBufAdvances(output, output')
     {
       output_size_estimate := header_size;
 
@@ -527,13 +534,14 @@ module Session {
     }
 
     method priv_try_encrypt_body(output: ByteBuf, input: ByteCursor) returns (result: Outcome, output': ByteBuf, input': ByteCursor)
+      requires Valid() && state == EncryptBody
       requires GoodByteBuf(output) && GoodByteCursor(input)
-      requires precise_size.Some? ==> data_so_far <= precise_size.get
-      requires alg_props != null && content_key != null
       modifies `output_size_estimate, `input_size_estimate, header`message_id, `data_so_far, `frame_seqno, `state, output.a
-      ensures result != AWS_OP_SUCCESS ==> state == old(state) && output' == output && input' == input
+      ensures Valid()
       ensures state == old(state) || state == WriteTrailer
-      ensures GoodByteBuf(output') && GoodByteCursor(input') && output'.a == output.a && input'.a == input.a
+      ensures ByteBufAdvances(output, output') && ByteCursorAdvances(input, input')
+      ensures unchanged(header`message_id) || fresh(header.message_id)
+      ensures result != AWS_OP_SUCCESS ==> state == old(state) && output' == output && input' == input
     {
       /* First, figure out how much plaintext we need. */
       var plaintext_size, frame_type;
@@ -623,12 +631,13 @@ module Session {
     }
 
     method priv_write_trailer(output: ByteBuf) returns (result: Outcome, output': ByteBuf)
+      requires Valid() && state == WriteTrailer
       requires GoodByteBuf(output)
-      requires alg_props != null
-      requires alg_props.signature_len != 0 ==> signctx != null
       modifies `input_size_estimate, `output_size_estimate, `signctx, `state, output.a
-      ensures result != AWS_OP_SUCCESS ==> state == old(state) && output' == output
+      ensures result == AWS_OP_SUCCESS ==> Valid()  // this means returns in a valid state only on success
       ensures state == old(state) || state == Done
+      ensures result != AWS_OP_SUCCESS ==> state == old(state) && output' == output
+      ensures ByteBufAdvances(output, output')
     {
       /* We definitely do not need any more input at this point.
        * We might need more output space, and if so we will update the
